Integrate side conditions into code generation

Optimizations/Canonicalizations/Common.thy
@@ -70,4 +70,206 @@ lemma well_formed_equal_defn [simp]:
   "well_formed_equal v\<^sub>1 v\<^sub>2 = (v\<^sub>1 \<noteq> UndefVal \<longrightarrow> v\<^sub>1 = v\<^sub>2)"
   unfolding well_formed_equal_def by simp
 
+
+subsection \<open>Condition Properties\<close>
+
+inductive_cases cond_Unary: "stampConditions (Unary op e) v"
+inductive_cases cond_Binary: "stampConditions (Binary op x y) v"
+inductive_cases cond_Const: "stampConditions (Constant x) y"
+inductive_cases cond_Value: "stampConditions (Value x) y"
+inductive_cases cond_ExprL: "stampConditions (Expr x) y"
+inductive_cases cond_ExprR: "stampConditions x (Expr y)"
+inductive_cases cond_Stamp: "stampConditions (Stamp x) y"
+inductive_cases cond_Combine: "stampConditions (Combine x y) v"
+inductive_cases cond_InstanceOf: "stampConditions (InstanceOf e c) y"
+inductive_cases cond_Method: "stampConditions (Method obj n p) y"
+inductive_cases cond_Method_stamp: "stampConditions (Method obj STR ''stamp'' p) y"
+inductive_cases cond_Method_upMask: "stampConditions (Method obj STR ''upMask'' p) y"
+inductive_cases cond_Method_mayBeSet: "stampConditions (Method obj STR ''mayBeSet'' p) y"
+inductive_cases cond_Method_downMask: "stampConditions (Method obj STR ''downMask'' p) y"
+inductive_cases cond_Method_mustBeSet: "stampConditions (Method obj STR ''mustBeSet'' p) y"
+inductive_cases cond_Method_lowerBound: "stampConditions (Method obj STR ''lowerBound'' p) y"
+inductive_cases cond_Method_upperBound: "stampConditions (Method obj STR ''upperBound'' p) y"
+lemmas cond_Method_cases = cond_Method_stamp cond_Method_upMask cond_Method_mayBeSet cond_Method_downMask cond_Method_mustBeSet cond_Method_lowerBound cond_Method_upperBound
+inductive_cases coerce_True: "coerce_to_bool c True"
+
+lemma logic_negation_bool:
+  assumes "is_IntVal val"
+  assumes "val_to_bool (unary_eval UnaryLogicNegation val)"
+  shows "\<not>(val_to_bool val)"
+  using assms unfolding unary_eval.simps intval_logic_negation.simps apply (cases val; auto)
+  by (metis logic_negate_def take_bit_of_0)
+
+lemma coerce_to_bool_det:
+  assumes "coerce_to_bool x c"
+  assumes "coerce_to_bool x c'"
+  shows "c = c'"
+  using assms apply (induction x c arbitrary: c' rule: coerce_to_bool.induct)
+  using coerce_to_bool.simps by blast+
+
+lemma stampConditions_det:
+  assumes "stampConditions x c"
+  assumes "stampConditions x c'"
+  shows "c = c'"
+  using assms apply (induction x c arbitrary: c' rule: stampConditions.induct) 
+  apply (metis Condition.inject(4) cond_Unary)
+  apply (metis Condition.inject(4) cond_Binary)
+  using cond_Const apply blast
+  using cond_Value apply blast 
+  using cond_ExprL apply blast 
+  using cond_Stamp apply blast 
+             apply (metis cond_Combine)
+            apply (smt (verit, best) Condition.distinct(71) Condition.inject(6) cond_InstanceOf)
+           apply (smt (verit, best) Condition.distinct(71) Condition.inject(6) cond_InstanceOf)
+  apply (smt (verit, best) Condition.inject(7) Condition.simps(82) cond_InstanceOf)
+  apply (smt (verit, best) Condition.inject(7) Condition.simps(82) cond_InstanceOf)
+  by (metis cond_Method_cases)+
+
+lemma instance_of_const:
+  assumes "evalCondition (InstanceOf (Expr x) STR ''ConstantNode'')"
+  shows "is_ConstantExpr x"
+proof -
+  obtain c' where c': "stampConditions (InstanceOf (Expr x) STR ''ConstantNode'') c' \<and> coerce_to_bool c' True"
+    using assms evalCondition_def by blast
+  then have "c' = (Value (IntVal 32 1))"
+    using assms coerce_True
+    by (smt (verit, ccfv_SIG) coerce_to_bool.intros(2) coerce_to_bool_det cond_InstanceOf val_to_bool.simps(1))
+  then have "class_name x = Some STR ''ConstantNode''"
+    using assms c'
+    by (meson Condition.inject(4) Value.inject(1) stampConditions.intros(5) stampConditions.intros(9) stampConditions_det zero_neq_one)
+  then show ?thesis
+    apply (cases x; auto)
+    subgoal for op e by (cases op; auto)
+    subgoal for op x y by (cases op; auto)
+    done
+qed
+
+lemma instance_of_not_const:
+  assumes "evalCondition (Unary UnaryLogicNegation (InstanceOf (Expr x) STR ''ConstantNode''))"
+  shows "\<not>(is_ConstantExpr x)"
+proof -
+  obtain val where val: "stampConditions (InstanceOf (Expr x) STR ''ConstantNode'') (Value val)"
+    using assms evalCondition_def
+    by (meson cond_Unary)
+  obtain c' where c': "stampConditions (Unary UnaryLogicNegation (InstanceOf (Expr x) STR ''ConstantNode'')) c' \<and> coerce_to_bool c' True"
+    using assms evalCondition_def by blast
+  then have "c' = Value (unary_eval UnaryLogicNegation val)"
+    by (meson stampConditions.intros(1) stampConditions_det val)
+  then have "val_to_bool (unary_eval UnaryLogicNegation val)"
+    using assms coerce_True c'
+    by (metis coerce_to_bool.intros(2) coerce_to_bool_det)
+  then have "\<not>(val_to_bool val)"
+    using logic_negation_bool
+    by (metis Value.disc(2) val_to_bool.elims(2))
+  then have "class_name x \<noteq> Some STR ''ConstantNode''"
+    using assms
+    using val stampConditions.intros(5) stampConditions.intros(8) stampConditions_det by fastforce
+  then show ?thesis
+    by (cases x; auto)
+qed
+
+lemma combine_cond_lhs:
+  assumes "evalCondition (x; y)"
+  shows "evalCondition x"
+  using assms using cond_Combine evalCondition_def
+  by (smt (z3) Condition.distinct(43) Condition.distinct(55) Condition.inject(8) coerce_to_bool.cases)
+
+lemma combine_cond_rhs:
+  assumes "evalCondition (x; y)"
+  shows "evalCondition y"
+  using assms using cond_Combine evalCondition_def
+  by (smt (z3) Condition.distinct(43) Condition.distinct(55) Condition.inject(8) coerce_to_bool.cases)
+
+abbreviation StampUnder :: "IRExpr \<Rightarrow> IRExpr \<Rightarrow> Condition" where
+  "StampUnder u v \<equiv> cond[(((Expr u)..stamp() instanceof IntegerStamp); 
+                          ((Expr v)..stamp() instanceof IntegerStamp)); 
+                          (((Expr u)..stamp()..upperBound()) < ((Expr v)..stamp()..lowerBound()))]"
+
+lemma stamp_Method:
+  shows "stampConditions ((Expr u)..stamp()) (Stamp (stamp_expr u))"
+  using stampConditions.intros(12) stampConditions.intros(5) stampConditions.intros(6) stamp_semantics by fastforce
+
+lemma stamp_upper_Method:
+  shows "stampConditions ((Stamp s)..upperBound()) (Value (IntVal 64 (word_of_int (stpi_upper s))))"
+  using stampConditions.intros(18) stampConditions.intros(3,6)
+  by (metis upperBound_of.simps upperBound_semantics)
+
+lemma stamp_lower_Method:
+  shows "stampConditions ((Stamp s)..lowerBound()) (Value (IntVal 64 (word_of_int (stpi_lower s))))"
+  using stampConditions.intros(17) stampConditions.intros(3,6)
+  by (metis lowerBound_of.simps lowerBound_semantics)
+
+lemma stamp_instanceof_IntegerStamp:
+  assumes "evalCondition cond[((Expr u)..stamp() instanceof IntegerStamp)]"
+  shows "is_IntegerStamp (stamp_expr u)"
+proof -
+  have "evalCondition cond[(Stamp (stamp_expr u)) instanceof IntegerStamp]"
+    using assms
+    by (smt (z3) evalCondition_def stampConditions.intros(10) stampConditions.intros(11) stampConditions.intros(6) stampConditions_det stamp_Method)
+  then have "stamp_class_name (stamp_expr u) = STR ''IntegerStamp''"
+    by (smt (verit, ccfv_threshold) assms coerce_to_bool.intros(2) coerce_to_bool_det evalCondition_def stampConditions.intros(11) stampConditions_det stamp_Method val_to_bool.simps(1))
+  then show ?thesis by (cases "stamp_expr u"; auto)
+qed
+
+no_notation ExclusiveOr ("_ ^ _")
+(*
+lemma stamp_upper_in_bounds:
+  assumes "valid_stamp u"
+  assumes "is_IntegerStamp u"
+  shows "(stpi_upper u) = (int_signed_value 64 (word_of_int (stpi_upper u)))"
+proof -
+  have "0 < stp_bits u \<and> stp_bits u \<le> 64"
+    by (metis Stamp.collapse(1) assms(1) assms(2) valid_stamp.simps(1))
+  then have "stpi_upper u \<ge> 2 ^ 64 div 2 * - 1"
+    using assms apply (induction "stp_bits u") 
+    apply simp using valid_stamp.simps bit_bounds.simps
+    using assms using valid_stamp.simps apply auto sorry
+    then show ?thesis
+      sorry
+  qed
+
+lemma stamp_lower_in_bounds:
+  assumes "valid_stamp u"
+  assumes "is_IntegerStamp u"
+  shows "(stpi_lower u) = (int_signed_value 64 (word_of_int (stpi_lower u)))"
+  sorry
+
+lemma stamp_under:
+  assumes "valid_stamp (stamp_expr u) \<and> valid_stamp (stamp_expr v)"
+  assumes "evalCondition cond[StampUnder u v]"
+  shows "stpi_upper (stamp_expr u) < stpi_lower (stamp_expr v)"
+proof -
+  have ec: "evalCondition cond[Value (IntVal 64 (word_of_int (stpi_upper (stamp_expr u)))) < Value (IntVal 64 (word_of_int (stpi_lower (stamp_expr v))))]" (is "evalCondition ?lowCond")
+    using assms combine_cond_lhs combine_cond_rhs
+    by (smt (z3) cond_Binary cond_Const cond_Method_lowerBound cond_Method_upperBound evalCondition_def lowerBound_of.simps lowerBound_semantics stampConditions.intros(2) stampConditions.intros(5) stampConditions_det stamp_Method upperBound_of.simps upperBound_semantics)
+  obtain val where val1: "stampConditions ?lowCond val \<and> coerce_to_bool val True"
+    using ec evalCondition_def by blast
+  have val2: "val = Value (bin_eval BinIntegerLessThan (IntVal 64 (word_of_int (stpi_upper (stamp_expr u)))) (IntVal 64 (word_of_int (stpi_lower (stamp_expr v)))))"
+    by (metis (no_types, lifting) BinaryCool Condition.inject(5) cond_Value val1)
+  have "... = Value (if (int_signed_value 64 (word_of_int (stpi_upper (stamp_expr u)))) < (int_signed_value 64 (word_of_int (stpi_lower (stamp_expr v)))) then IntVal 32 1 else IntVal 32 0)"
+    unfolding bin_eval.simps intval_less_than.simps bool_to_val_bin.simps using bool_to_val.simps by auto
+  also have "val = Value (IntVal 32 1)"
+    using calculation coerce_True val1 val2 by fastforce
+  ultimately have lt: "(int_signed_value 64 (word_of_int (stpi_upper (stamp_expr u)))) < (int_signed_value 64 (word_of_int (stpi_lower (stamp_expr v))))"
+    using Value.inject(1) val2 by fastforce
+  have isu: "is_IntegerStamp (stamp_expr u)"
+    by (meson assms(2) combine_cond_lhs stamp_instanceof_IntegerStamp)
+  have isv: "is_IntegerStamp (stamp_expr v)"
+    using assms(2) combine_cond_lhs combine_cond_rhs stamp_instanceof_IntegerStamp by blast
+  have ueq: "stpi_upper (stamp_expr u) = int_signed_value 64 (word_of_int (stpi_upper (stamp_expr u)))"
+    using assms(1) isu stamp_upper_in_bounds by blast
+  have veq: "stpi_lower (stamp_expr v) = int_signed_value 64 (word_of_int (stpi_lower (stamp_expr v)))"
+    using assms(1) isv stamp_lower_in_bounds by blast
+  from lt show ?thesis
+    using ueq veq assms by argo
+qed
+
+lemma stamp_under_lower:
+  assumes "valid_stamp (stamp_expr u) \<and> valid_stamp (stamp_expr v)"
+  assumes "evalCondition (StampUnder u v)"
+  shows "stamp_under (stamp_expr u) (stamp_expr v)"
+  using assms
+  by (smt (verit, best) Stamp.collapse(1) combine_cond_lhs combine_cond_rhs stamp_instanceof_IntegerStamp stamp_under stamp_under.simps(1))
+*)
+
 end
